\documentclass{article}

% Maths
\usepackage{amsmath}

% Hyperlink
\usepackage{hyperref}
\hypersetup{
    colorlinks=true,
    linkcolor=blue,
    filecolor=magenta,      
    urlcolor=cyan,
    pdfpagemode=FullScreen,
}

% Figures
\usepackage{graphics, float, subfig}
\usepackage[pdflatex]{graphicx}

% Itemize
\renewcommand{\labelitemi}{\textbullet}
\renewcommand{\labelitemii}{\textbullet}
\renewcommand{\labelitemiii}{\textbullet}

% Margins
\usepackage[margin=1in]{geometry}

% Helpful commands
\newcommand{\x}{\mathbf{x}}
\newcommand{\A}{\mathbf{A}}
\newcommand{\B}{\mathbf{b}} % \b already defined
\newcommand{\I}{\mathbf{I}}

\begin{document}

% TODO: Make a nice title page
APPM 4600 Project 3: Regularization in Least Squares\\
Alexey Yermakov, Logan Barnhart, and Tyler Jensen

\section{Ridge Regression}
\subsection{Deriving the Ridge Estimator}

Recalling that $||\mathbf{x}||_{2}^{2}=\mathbf{x}^T \mathbf{x}$, we'll rewrite $||\mathbf{Ax}-\mathbf{b}||_{2}^{2} + \gamma||\mathbf{x}||_{2}^{2}$:

\begin{equation} \label{eqn:rls}
    \arg \max_{x} ||\A\x-\B||_{2}^{2} + \gamma||\x||_{2}^{2}
\end{equation}

\begin{equation*}
\begin{split}
    & ||\A\x-\B||_{2}^{2} + \gamma||\x||_{2}^{2} =\\
    & =  (\A\x - \B)^T (\A\x - \B) + \gamma \x^T \x \\ 
    & =  ((\A\x)^T - \B^T) (\A\x - \B) + \gamma \x^T \x \\ 
    & =  (\x^T\A^T - \B^T) (\A\x - \B) + \gamma \x^T \x \\ 
    & = \x^T \A^T \A\x - \x^T \A^T \B - \B^T \A\x + \B^T \B + \gamma \x^T \x
\end{split}
\end{equation*}

Before we proceed further, I'll define what $\A$, $\B$, and $\x$ are. We want a least-squares fit to an $m$-degree polynomial $p_m(x)=a_0+a_1*x+\ldots+a_m*x^m$ where we have $n$ data points $\{x_0,b_0\}$. To have our system be overdetermined, we also assume $n > m$.

\begin{equation*}
    \A =
    \begin{bmatrix}
        1 & x_0 & x_0 ^2 & \ldots & x_0^m \\
        1 & x_1 & x_1 ^2 & \ldots & x_1^m \\
        1 & x_2 & x_2 ^2 & \ldots & x_2^m \\
        \vdots & \vdots & \vdots & \ddots & \vdots \\
        1 & x_n & x_n ^n & \ldots & x_n^m \\
    \end{bmatrix}
    \quad
    \x =
    \begin{bmatrix}
        a_0\\
        a_1\\
        \vdots\\
        a_m
    \end{bmatrix}
    \quad
    \B =
    \begin{bmatrix}
        b_0\\
        b_1\\
        \vdots\\
        b_n
    \end{bmatrix}
\end{equation*}

Where $dim(\A)=(n+1)\times(m+1)$, $dim(\x)=(m+1)\times(1)$, and $dim(\B)=(n+1)\times(1)$.

$ $ %Newline

I'll now prove $\x^T\A^T\B = \B^T\A\x$. Note first that $(\B^T\A\x)^T=\x^T\A^T\B$. Further, $dim(\x^T\A^T\B) = (1) \times (1) = dim(\B^T\A\x)$. Also, note that the transpose of a $1 \times 1$ matrix is the same matrix: $[c]^T=[c]$. It then follows that $\x^T\A^T\B = \B^T\A\x$, completing the proof.

$ $ %Newline

So,

\begin{equation} \label{eqn:rls_prod}
\begin{split}
    &\x^T \A^T \A\x - \x^T \A^T \B - \B^T \A\x + \B^T \B + \gamma \x^T \x = \\ 
    & = \x^T \A^T \A\x -2 \B^T \A\x + \B^T \B + \gamma \x^T \x\\
    & = (\A\x)^T(\A\x) -2 \B^T \A\x + \B^T \B + \gamma \x^T \x
\end{split}
\end{equation}

Now, I'll show what each of the above values (since each matrix is $1 \times 1$, meaning it's a scalar) actually is:

\begin{equation} \label{eqn:Ax}
\begin{split}
    & \A\x = \\
    & =
    \begin{bmatrix}
        1 & x_0 & x_0 ^2 & \ldots & x_0^m \\
        1 & x_1 & x_1 ^2 & \ldots & x_1^m \\
        1 & x_2 & x_2 ^2 & \ldots & x_2^m \\
        \vdots & \vdots & \vdots & \ddots & \vdots \\
        1 & x_n & x_n ^n & \ldots & x_n^m \\
    \end{bmatrix}
    \times
    \begin{bmatrix}
        a_0\\
        a_1\\
        \vdots\\
        a_m
    \end{bmatrix}\\
    & =
    \begin{bmatrix}
        a_0 + a_1 x_0 + a_2 x_0 ^2 + \ldots + a_m x_0^m \\
        a_0 + a_1 x_1 + a_2 x_1 ^2 + \ldots + a_m x_1^m \\
        a_0 + a_1 x_2 + a_2 x_2 ^2 + \ldots + a_m x_2^m \\
        \vdots \\
        a_0 + a_1 x_n + a_2 x_n ^2 + \ldots + a_m x_n^m \\
    \end{bmatrix}
\end{split}
\end{equation}

Then, $(\A\x)^T \A\x$ is just a simple inner product (we will use the result from \ref{eqn:Ax}):

\begin{equation} \label{eqn:axtax}
\begin{split}
    & (\A\x)^T \A\x = \\
    & =
    \begin{bmatrix}
        a_0 + a_1 x_0 + a_2 x_0 ^2 + \ldots + a_m x_0^m \\
        a_0 + a_1 x_1 + a_2 x_1 ^2 + \ldots + a_m x_1^m \\
        a_0 + a_1 x_2 + a_2 x_2 ^2 + \ldots + a_m x_2^m \\
        \vdots \\
        a_0 + a_1 x_n + a_2 x_n ^2 + \ldots + a_m x_n^m \\
    \end{bmatrix} ^T
    \times
    \begin{bmatrix}
        a_0 + a_1 x_0 + a_2 x_0 ^2 + \ldots + a_m x_0^m \\
        a_0 + a_1 x_1 + a_2 x_1 ^2 + \ldots + a_m x_1^m \\
        a_0 + a_1 x_2 + a_2 x_2 ^2 + \ldots + a_m x_2^m \\
        \vdots \\
        a_0 + a_1 x_n + a_2 x_n ^2 + \ldots + a_m x_n^m \\
    \end{bmatrix} \\
    & = (a_0 + a_1 x_0 + \ldots + a_m x_0^m)^ 2 + (a_0 + a_1 x_1 + \ldots + a_m x_1^m)^ 2\\
    & + \ldots + (a_0 + a_1 x_n + \ldots + a_m x_n^m)^ 2
\end{split}
\end{equation}

\begin{equation} \label{eqn:2bax}
\begin{split}
    & 2 \B ^T \A \x = \\
    & = 2 \times
    \begin{bmatrix}
        b_0 &
        b_1 &
        \ldots & 
        b_n
    \end{bmatrix}
    \times
    \begin{bmatrix}
        1 & x_0 & x_0 ^2 & \ldots & x_0^m \\
        1 & x_1 & x_1 ^2 & \ldots & x_1^m \\
        1 & x_2 & x_2 ^2 & \ldots & x_2^m \\
        \vdots & \vdots & \vdots & \ddots & \vdots \\
        1 & x_n & x_n ^n & \ldots & x_n^m \\
    \end{bmatrix}
    \times
    \begin{bmatrix}
        a_0\\
        a_1\\
        \vdots\\
        a_m
    \end{bmatrix}\\
    & = 2 \times
    \begin{bmatrix}
        b_0 + b_1 + b_2 + \ldots + b_n \\
        b_0 x_0 + b_1 x_1 + b_2 x_2 + \ldots + b_n x_n \\
        b_0 x_0^2 + b_1 x_1^2 + b_2 x_2^2 + \ldots + b_n x_n^2 \\
        \vdots\\
        b_0 x_0^m + b_1 x_1^m + b_2 x_2^m + \ldots + b_n x_innern^m \\
    \end{bmatrix} ^T
    \times
    \begin{bmatrix}
        a_0\\
        a_1\\
        \vdots\\
        a_m
    \end{bmatrix}\\
    & = 2(a_0 (b_0 + b_1 + \ldots + b_n) + a_1 (b_0 x_0 + b_1 x_1 + \ldots + b_n x_n) + \ldots + a_m (b_0 x_0^m + b_1 x_1^m + \ldots + b_n x_n^m))
\end{split}
\end{equation}

\begin{equation} \label{eqn:gxx}
\begin{split}
    & \gamma \x ^T \x = \\
    & \text{This is a simple inner product multiplied by a scalar} \\
    & = \gamma a_0 ^2 + \gamma a_1 ^2 + \ldots + \gamma a_m^2
\end{split}
\end{equation}

Great! Now lets take the derivates of \ref{eqn:axtax}, \ref{eqn:2bax}, and \ref{eqn:gxx} with respect to $\x$ to get the derivative of \ref{eqn:rls} with respect to $\x$. In effect, we'll get a vector where the $i$-th element is the derivative of \ref{eqn:rls} with respect to $a_i$.

First, let's take the derivatives of \ref{eqn:axtax}:

\begin{equation}
\begin{split}
    & \frac{d}{d\x} (\A\x)^T \A\x = \\
    & =
    \begin{bmatrix}
        \frac{d}{d a_0} (\A\x)^T \A\x \\
        \frac{d}{d a_1} (\A\x)^T \A\x \\
        \vdots \\
        \frac{d}{d a_m} (\A\x)^T \A\x \\
    \end{bmatrix}\\
    & =
    \begin{bmatrix}
        2(a_0 + a_1 x_0 + \dots + a_m x_0 ^ m) + 2(a_0 + a_1 x_1 + \dots + a_m x_1 ^ m) + \ldots + 2(a_0 + a_1 x_n + \dots + a_m x_n ^ m)\\
        2 x_0(a_0 + a_1 x_0 + \dots + a_m x_0 ^ m) + 2 x_1(a_0 + a_1 x_1 + \dots + a_m x_1 ^ m) + \ldots + 2 x_n(a_0 + a_1 x_n + \dots + a_m x_n ^ m)\\
        \vdots \\
        2 x_0^m(a_0 + a_1 x_0 + \dots + a_m x_0 ^ m) + 2 x_1^m(a_0 + a_1 x_1 + \dots + a_m x_1 ^ m) + \ldots + 2 x_n^m(a_0 + a_1 x_n + \dots + a_m x_n ^ m)
    \end{bmatrix}\\
    & = 2 \times
    \begin{bmatrix}
        a_0 \sum_{i=0}^{n} 1 + a_1 \sum_{i=0}^{n} x_i + a_2 \sum_{i=0}^{n} x_i^2 + \ldots + a_m \sum_{i=0}^{n} x_i ^ m\\
        a_0 \sum_{i=0}^{n} x_i + a_1 \sum_{i=0}^{n} x_i^2 + a_2 \sum_{i=0}^{n} x_i^3 + \ldots + a_m \sum_{i=0}^{n} x_i ^ {m+1}\\
        \vdots \\
        a_0 \sum_{i=0}^{n} x_i^m + a_1 \sum_{i=0}^{n} x_i^{m+1} + a_2 \sum_{i=0}^{n} x_i^{m+2} + \ldots + a_m \sum_{i=0}^{n} x_i ^ {2m}\\
    \end{bmatrix}\\
    & = 2 \times
    \begin{bmatrix}
        \sum_{i=0}^{n} 1 & \sum_{i=0}^{n} x_i & \sum_{i=0}^{n} x_i ^2 & \ldots & \sum_{i=0}^{n} x_i ^m\\
        \sum_{i=0}^{n} x_i & \sum_{i=0}^{n} x_i ^2 & \sum_{i=0}^{n} x_i ^3 & \ldots & \sum_{i=0}^{n} x_i ^m\\
        \sum_{i=0}^{n} x_i ^2 & \sum_{i=0}^{n} x_i ^3 & \sum_{i=0}^{n} x_i ^4 & \ldots & \sum_{i=0}^{n} x_i ^m\\
        \vdots & \vdots & \vdots & \ddots & \vdots \\
        \sum_{i=0}^{n} x_i ^{m} & \sum_{i=0}^{n} x_i ^{m+1} & \sum_{i=0}^{n} x_i ^{m+2} & \ldots & \sum_{i=0}^{n} x_i ^{2m}
    \end{bmatrix}
    \times
    \begin{bmatrix}
        a_0 \\
        a_1 \\
        a_2 \\
        \vdots \\
        a_m
    \end{bmatrix}\\
    & = 2 \times
    \begin{bmatrix}
        1 & 1 & 1 & \ldots & 1 \\
        x_0 & x_1 & x_2 & \ldots & x_n \\
        x_0^2 & x_1^2 & x_2 ^2 & \ldots & x_n^2 \\
        \vdots & \vdots & \vdots & \ddots & \vdots \\
        x_0^m & x_1^m & x_2 ^m & \ldots & x_n^m \\
    \end{bmatrix}
    \times
    \begin{bmatrix}
        1 & x_0 & x_0 ^2 & \ldots & x_0^m \\
        1 & x_1 & x_1 ^2 & \ldots & x_1^m \\
        1 & x_2 & x_2 ^2 & \ldots & x_2^m \\
        \vdots & \vdots & \vdots & \ddots & \vdots \\
        1 & x_n & x_n ^n & \ldots & x_n^m \\
    \end{bmatrix}
    \times
    \begin{bmatrix}
        a_0 \\
        a_1 \\
        a_2 \\
        \vdots \\
        a_m
    \end{bmatrix}\\
    &= 2\A ^T \A \x
\end{split}
\end{equation}

Secondly, let's take the derivatives of \ref{eqn:2bax}:

\begin{equation}
\begin{split}
    & \frac{d}{d\x} 2 \B ^T \A \x = \\
    & =
    \begin{bmatrix}
        \frac{d}{d a_0} 2 \B ^T \A \x \\
        \frac{d}{d a_1} 2 \B ^T \A \x \\
        \vdots \\
        \frac{d}{d a_m} 2 \B ^T \A \x \\
    \end{bmatrix}\\
    & = 2 \times
    \begin{bmatrix}
        b_0 + b_1 + \ldots + b_n \\
        b_0x_0 + b_1x_1 + \ldots + b_nx_n \\
        b_0x_0^2 + b_1x_1^2 + \ldots + b_nx_n^2 \\
        \vdots \\
        b_0x_0^m + b_1x_1^m + \ldots + b_nx_n^m \\
    \end{bmatrix}\\
    &= 2 \times
    \begin{bmatrix}
        1 & 1 & 1 & \ldots & 1 \\
        x_0 & x_1 & x_2 & \ldots & x_n \\
        x_0^2 & x_1^2 & x_2 ^2 & \ldots & x_n^2 \\
        \vdots & \vdots & \vdots & \ddots & \vdots \\
        x_0^m & x_1^m & x_2 ^m & \ldots & x_n^m
    \end{bmatrix}
    \times
    \begin{bmatrix}
        b_0\\
        b_1\\
        \vdots\\
        b_n
    \end{bmatrix}\\
    &= 2 \A ^T \B
\end{split}
\end{equation}

Lastly, let's take the derivatives of \ref{eqn:gxx}:

\begin{equation}
\begin{split}
    & \frac{d}{d\x} \gamma \x^T \x = \\
    & =
    \begin{bmatrix}
        \frac{d}{d a_0} \gamma \x^T \x \\
        \frac{d}{d a_1} \gamma \x^T \x \\
        \vdots \\
        \frac{d}{d a_m} \gamma \x^T \x \\
    \end{bmatrix}\\
    &= \gamma \times
    \begin{bmatrix}
        2 a_0 \\
        2 a_1 \\
        2 a_2 \\
        \vdots \\
        2 a_m
    \end{bmatrix}\\
    &= 2 \times \gamma \times
    \begin{bmatrix}
        1 & 0 & 0 & \ldots & 0\\
        0 & 1 & 0 & \ldots & 0\\
        0 & 0 & 1 & \ldots & 0\\
        \vdots & \vdots & \vdots & \ddots & \vdots \\
        0 & 0 & 0 & \ldots & 1\\
    \end{bmatrix}
    \times
    \begin{bmatrix}
        a_0 \\
        a_1 \\
        a_2 \\
        \vdots \\
        a_m
    \end{bmatrix}\\
    &= 2 \gamma \I \x
\end{split}
\end{equation}

Now we can recall \ref{eqn:rls_prod} and note that to find the minimum of the least squares equation given by \ref{eqn:rls} we can find where the derivative of \ref{eqn:rls_prod} is equal to zero:

\begin{equation}
\begin{split}
    \frac{d}{d \x} (\frac{}{}(\A\x)^T(\A\x) -2 \B^T \A\x + \B^T \B + \gamma \x^T \x) &= 0 \\
    2 \A ^T \A \x - 2 \A ^T \B + 2 \gamma \I \x &= 0 \\
    \A ^T \A \x - \A ^T \B + \gamma \I \x &= 0 \\
    \A ^T \A \x + \gamma \I \x - \A ^T \B &= 0 \\
    ( \A ^T \A + \gamma \I ) \x - \A ^T \B &= 0 \\
    ( \A ^T \A + \gamma \I ) \x  &= \A ^T \B \\
    \x &= ( \A ^T \A + \gamma \I )^{-1} \A ^T \B  \\
\end{split}
\end{equation}

We have now arrived at the equation for Ridge Regression! We note that there is a typo in the project description for the equation $E_{ridge}=( \A ^T \A + \gamma \I )^{-1} \A ^T$, where there is no trailing $\B$.

\end{document}